Progress on Preservation Proof, slight rework of SubstitutionPreservesTyping * Added a new induction principle for Terms and Bindings that returns a 	Prop instead of Type. * Facts that follow from SubstitutionPreservesTyping are now nicely separated

src/Language/PlutusIR/Semantics/TypeSafety/Preservation.v
@@ -8,13 +8,46 @@ Require Import PlutusCert.Language.PlutusIR.Semantics.Dynamic.BuiltinMeanings.
 Require Import PlutusCert.Language.PlutusIR.Semantics.TypeSafety.SubstitutionPreservesTyping.
 
 
-Lemma preservation__eval_defaultfun : forall ctx t T,
-    ctx = emptyContext ->
-    ctx |-+ t : T ->
+Lemma preservation__compute_defaultfun : forall t T,
+    emptyContext |-+ t : T ->
     forall v,
       compute_defaultfun t = Datatypes.Some v ->
-      ctx |-+ v : T.
-Proof. Admitted. (* TODO *)
+      emptyContext |-+ v : T.
+Proof.
+  intros.
+  destruct t; inversion H0.
+  destruct t1; inversion H0. {
+    destruct t1_1; inversion H0. {
+      destruct t1_1_1; inversion H0. 
+      destruct d; inversion H0.
+      destruct t1_1_2; inversion H0.
+      destruct s; inversion H0.
+      destruct u; inversion H0.
+      destruct v0; inversion H0.
+      destruct t1_2; inversion H0.
+      destruct s; inversion H0.
+      destruct u0; inversion H0.
+      destruct v0; inversion H0.
+      destruct t2; inversion H0.
+      destruct s; inversion H0.
+      destruct u1; inversion H0.
+      destruct v0; inversion H0.
+      inversion H. subst.
+      inversion H23; subst.
+      apply Eqdep.EqdepTheory.inj_pair2 in H20.
+      subst.
+      inversion H21; subst.
+      inversion H24; subst.
+      apply Eqdep.EqdepTheory.inj_pair2 in H22.
+      subst.
+      inversion H20; subst.
+      inversion H26; subst.
+      apply Eqdep.EqdepTheory.inj_pair2 in H25.
+      subst.
+      inversion H22; subst.
+      apply T_Constant.
+    }
+Admitted. (* TODO *)
 
 Theorem unique_kinds : forall ctx T K K',
     ctx |-* T : K ->
@@ -23,171 +56,196 @@ Theorem unique_kinds : forall ctx T K K',
 Proof. Admitted.
 
 
-Definition P_term (ctx : Context) t T := 
-  ctx = emptyContext ->
-  forall v, 
-    t ==> v -> 
-    ctx |-+ v : T.
+Definition P_eval (t v : Term) :=
+  forall T,
+    emptyContext |-+ t : T ->
+    emptyContext |-+ v : T.
 
+Definition P_eval_bindings_nonrec (t v : Term) :=
+  forall bs t0,
+    t = Let NonRec bs t0 ->
+    forall T,
+      emptyContext |-+ t : T ->
+      emptyContext |-+ v : T.
 
-Definition P_constructor ctx c := ctx |-ok_c c.
+Definition P_eval_bindings_rec (bs0 : list Binding) (t v : Term) :=
+  forall bs t0,
+    t = Let Rec bs t0 ->
+    forall T,
+      emptyContext |-+ t : T ->
+      emptyContext |-+ v : T.
 
-Definition P_bindings_nonrec ctx bs := 
-  ctx = emptyContext ->
-  forall t0 T v0,
-    ctx |-oks_nr bs ->    
-    P_term (append (flatten (List.map binds bs)) ctx) t0 T ->
-    eval_bindings_nonrec (Let NonRec bs t0) v0 ->
-    append (flatten (List.map binds bs)) ctx |-+ t0 : T ->
-    ctx |-+ v0 : T.
-
-Definition P_bindings_rec ctx bs := ctx |-oks_r bs.
-
-Definition P_binding ctx b := (*ctx |-ok b.*)
-  forall s x Tb tb vb t t' T,
-    b = TermBind s (VarDecl x Tb) tb ->
-    (append (binds (TermBind s (VarDecl x Tb) tb)) ctx) |-+ t : T ->
-    substitute x vb t t' ->
-    ctx |-+ t' : T.
 
 Axiom skip : forall P, P.
 
-Theorem preservation' : forall (ctx : Context) (t : Term) (T : Ty),
-  ctx |-+ t : T ->
-  P_term ctx t T. 
+Lemma e : forall T T3 T2 T1 T0,
+  substituteT "a" T (Ty_Fun (Ty_Builtin (Some (TypeIn DefaultUniBool))) (Ty_Fun (Ty_Var "a") (Ty_Fun (Ty_Var "a") (Ty_Var "a")))) =b
+    Ty_Fun T3 (Ty_Fun T2 (Ty_Fun T1 T0)) -> 
+  T1 =b T2.
 Proof.
-  apply has_type__ind with (P := P_term) (P0 := P_constructor) (P1 := P_bindings_nonrec) (P2 := P_bindings_rec) (P3 := P_binding).
-  - intros. unfold P_term. intros. 
-    subst.
-    inversion H5; subst.
-    unfold P_bindings_nonrec in H1.
-    eapply H1.
-    + reflexivity.
-    + assumption.
-    + apply H3.
-    + apply H7.
-    + apply H2.
-  - apply skip. (* TODO *)
-  - (* T_Var *)
-    intros. unfold P_term. intros.
-    inversion H1. 
-  - (* T_TyAbs *)
-    intros. unfold P_term. intros.
-    inversion H2. subst.
+  intros.
+  simpl in H.
+  induction H; auto.
+  - apply skip.
+  - apply skip.
+Qed.
+
+
+Theorem preservation' : 
+  (forall (t v : Term), t ==> v -> P_eval t v) /\
+  (forall (t v : Term), eval_bindings_nonrec t v -> P_eval_bindings_nonrec t v) /\
+  (forall (bs0 : list Binding) (t v : Term), eval_bindings_rec bs0 t v -> P_eval_bindings_rec bs0 t v). 
+Proof.
+  apply eval__multind with
+    (P := P_eval)
+    (P0 := P_eval_bindings_nonrec)
+    (P1 := P_eval_bindings_rec).
+  - intros. unfold P_eval. intros.
+    eapply H0; eauto.
+  - intros. unfold P_eval. intros.
+    eapply H0; eauto.
+  - (* E_TyAbs *)
+    intros. unfold P_eval. intros.
+    inversion H1. subst.
     apply T_TyAbs.
     apply skip.
-  - (* T_LamAbs *)
-    intros. unfold P_term. intros.
-    inversion H3. subst.
-    apply T_LamAbs.
-    + assumption.
-    + assumption.
-  - (* T_Apply *) 
-    intros. unfold P_term. intros.
-    inversion H4.
-    + subst. 
-      apply H0 in H7; auto. 
-      apply H2 in H8; auto.
-      
-      inversion H7. subst.  eapply substitution_preserves_typing in H9; eauto. apply skip. (* TODO *)
-    + subst. 
-      apply T_Apply with T1.
-      * apply H0; auto.
-      * apply H2; auto.
-    + subst.
-      apply preservation__eval_defaultfun with (Apply v1 v2); auto.
-      apply T_Apply with T1.
-      -- apply H0; auto.
-      -- apply H2; auto.
-    + subst.
-      eapply T_Apply; eauto.
-    + subst.
-      eapply T_Apply; eauto.
-    + subst.
-      apply skip.
-    + subst.
-      apply skip.
-  - (* T_Constant *)
-    intros. unfold P_term. intros.
-    inversion H0. subst.
-    apply T_Constant.
-  - (* T_Builtin *)
-    intros. unfold P_term. intros.
-    inversion H0. subst.
-    apply T_Builtin.
-  - (* T_TyInst *) 
-    intros. unfold P_term. intros.
-    inversion H4.
-    + subst.
-      apply T_TyInst with (T1 := T1) (X := X) (K2 := K2).
-      * apply H0; auto.
-      * assumption.
-      * assumption.
-    + subst. apply skip. (* TODO *)
-  - (* T_Error *)
-    intros. unfold P_term. intros.
-    inversion H1. subst.
-    apply T_Error.
-    assumption.
-  - (* T_IWrap *)
-    intros. unfold P_term. intros.
-    inversion H5. subst.
-    apply T_IWrap with (X := X) (K := K) (S := S).
-    + assumption.
-    + apply H1; auto.
-    + assumption.
-    + assumption.
-  - (* T_Unwrap *)
-    intros. unfold P_term. intros.
-    inversion H4. subst.
-    apply H0 in H6 as H7.
-    inversion H7. subst.
-    assert (K = K0) by eauto using unique_kinds.
-    subst. (* TODO: something with transitivity and free variables *)
-    apply skip.
-    reflexivity.
-
-  - (* W_Con *)
-    intros. unfold P_constructor. 
-    apply W_Con.
-    assumption.
-
-  - intros. unfold P_bindings_nonrec. intros.
-    inversion H2. subst.
-    simpl in H3.
-    unfold P_term in H1.
-    simpl in H1.
-    rewrite flatten_nil in H1.
-    rewrite append_emptyContext_l in H1.
-    apply H1; auto.
-  - intros. unfold P_bindings_nonrec. unfold P_bindings_nonrec in H2. intros.
+  - intros. unfold P_eval. intros.
+    assumption. 
+  - intros. unfold P_eval. intros.
     inversion H6. subst.
+    apply H0 in H10.
+    apply H2 in H12.
+    eapply substitution_preserves_typing in H3; eauto.
+    inversion H10. subst.
+    eauto.
+  - intros. unfold P_eval. intros.
+    assumption.
+  - intros. unfold P_eval. intros.
+    assumption.
+  - intros. unfold P_eval. intros.
+    inversion H5. subst.
+    apply T_Apply with T1.
+    + apply H0.
+      assumption. 
+    + apply H3.
+      assumption.
+  - intros. unfold P_eval. intros.
+    inversion H6. subst.
+    eapply preservation__compute_defaultfun.
+    + apply T_Apply with T1. 
+      * apply H0.
+        assumption.
+      * apply H3.
+        assumption.
+    + assumption.
+  - intros. unfold P_eval. intros.
+    inversion H1; subst.
+    eapply T_TyInst; eauto.
+  - intros. unfold P_eval. intros.
+    inversion H3; subst.
+    eapply T_Apply; eauto.
+  - intros. unfold P_eval. intros.
+    inversion H1; subst.
+    eapply T_Apply; eauto.
+  - intros. unfold P_eval. intros.
+    inversion H3; subst.
+    apply H0 in H7.
+    apply H2.
 
-    eapply H0.
+    inversion H7. subst.
+    inversion H8. subst.
+    inversion H10; subst.
+    inversion H6. subst.
+    simpl in H16.
+    
+    apply skip. (* TODO *)
+  - intros. unfold P_eval. intros.
+    inversion H3. subst.
+    apply H0 in H7.
+    apply H2.
+
+    inversion H7. subst.
+    inversion H8. subst.
+    inversion H10. subst.
+    inversion H6. subst.
+    simpl in H16.
+
+    apply skip. (* TODO *)
+  - intros. unfold P_eval. intros.
+    inversion H1. subst.
+    apply skip. (* TODO *)
+  - intros. unfold P_eval. intros.
+    assumption.
+  - intros. unfold P_eval. intros.
+    inversion H1. subst.
+    eapply T_IWrap; eauto.
+  - intros. unfold P_eval. intros.
+    inversion H1. subst.
+    apply H0 in H3.
+    inversion H3. subst.
+    apply skip. (* TODO *)
+
+  - (* E_NilB_NonRec *)
+    intros. unfold P_eval_bindings_nonrec. intros.
+    inversion H1. subst.
+    inversion H2. subst.
+    simpl in H9.
+    rewrite flatten_nil in H9.
+    rewrite append_emptyContext_l in H9.
+    apply H0.
+    assumption.
+  - (* E_ConsB_NonRec *)
+    intros. unfold P_eval_bindings_nonrec. intros.
+    inversion H5. subst.
+    inversion H6. subst.
+    eapply H4.
     + reflexivity.
-    + simpl.
-      eapply H2.
-      * (*
-      * assumption.
-      * unfold flatten in H5.
-        unfold flatten in H5.
-        unfold append in H5.
-        simpl in H5. unfold extendT in H5. simpl in H5. (*
-        rewrite List.concat_app in H5. simpl in H5.
-        rewrite <- List.app_assoc in H5. simpl in H5.
-        apply H5.
-      * apply skip. 
-      * unfold flatten in H7.
-        unfold flatten in H7.
-        unfold append in H7.
-        simpl in H7. unfold extendT in H7. simpl in H7.
-        rewrite List.concat_app in H7. simpl in H7.
-        rewrite <- List.app_assoc in H7. simpl in H7.
-        apply H7.*)*)
+    + eapply T_Let.
+      * reflexivity.
+      * eapply substitution_preserves_typing__Bindings_NonRec.
+        -- inversion H11. subst.
+           simpl in H12.
+           rewrite append_emptyContext_r in H12.
+           apply H12.
+        -- inversion H11. subst.
+           inversion H10. subst.
+           apply H0.
+           assumption.
+        -- assumption.
+      * eapply substitution_preserves_typing.
+        -- simpl in H13.
+           erewrite <- append_extendT_permute.
+           ++ rewrite flatten_extract in H13.
+              rewrite append_emptyContext_r in H13.
+              assert (List.map binds bs = List.map binds bs'). {
+                eapply substitution_preserves_typing__Bindings_NonRec.
+                - inversion H11. subst.
+                  simpl in H12.
+                  rewrite append_emptyContext_r in H12.
+                  apply H12.
+                - inversion H11. subst.
+                  inversion H10. subst.
+                  apply H0.
+                  assumption.
+                - assumption.
+              }
+              rewrite <- H7.
+              apply H13.
+           ++ apply skip. (* TODO *)
+        -- inversion H11. subst.
+           inversion H10. subst.
+           apply H0.
+           assumption.
+        -- assumption.
+
+  - (* E_NilB_Rec *)
+    intros. unfold P_eval_bindings_rec. intros.
+    inversion H1. subst.
+    
 Abort.
 
 Theorem preservation : forall t v T,
     emptyContext |-+ t : T ->
     t ==> v ->
     emptyContext |-+ v : T.
-Proof. Admitted.
+Proof. Abort.
