src/Util.v
@@ -47,6 +47,30 @@ Definition ForallT_tl {A P} {x : A} {xs} : ForallT P (x :: xs) -> ForallT P xs :
     | ForallT_cons p ps => ps
   end.
 
+(* ForallT for Props *)  
+Inductive ForallP (A : Type) (P : A -> Prop) : list A -> Prop :=
+  | ForallP_nil : ForallP P nil
+  | ForallP_cons : forall {x : A} {l : list A},
+                  P x -> ForallP P l -> ForallP P (x :: l).
+Arguments ForallP_nil {_} {_}.
+Arguments ForallP_cons {_} {_} {_} {_}.
+#[export] Hint Constructors ForallP : core.
+
+Definition ForallP_uncons {A P} {x : A} {xs} : ForallP P (x :: xs) -> (P x * ForallP P xs) :=
+  fun ps => match ps with
+    | ForallP_cons p ps => (p, ps)
+  end.
+
+Definition ForallP_hd {A P} {x : A} {xs} : ForallP P (x :: xs) -> P x :=
+  fun ps => match ps with
+    | ForallP_cons p _ps => p
+  end.
+
+Definition ForallP_tl {A P} {x : A} {xs} : ForallP P (x :: xs) -> ForallP P xs :=
+  fun ps => match ps with
+    | ForallP_cons p ps => ps
+  end.
+
 
 (* Prove P or Q depending on x *)
 Definition sumboolOut (P Q : Prop) (x : {P} + {Q}) :=
